Foundation/Modal/Kripke2/Logic/K.lean
@@ -11,15 +11,14 @@ variable {α : Type u} {φ : Formula α}
 
 namespace K
 
-theorem kripke_sound : Modal.K _ ⊢ φ → (∀ {κ}, [Nonempty κ] → ∀ F : Rel κ κ, ∀ V, (⟨F, V⟩ : KripkeModel κ α) ⊧ φ)
-  := by
+theorem kripke_sound : Modal.K _ ⊢ φ → (∀ κ, [Nonempty κ] → ∀ F, ∀ V, (⟨F, V⟩ : KripkeModel κ α) ⊧ φ) := by
   intro h κ _ F;
   apply Hilbert.Normal.valid_of_provable2 F ?_ h;
   rintro V _ ⟨_, _, rfl⟩;
   exact KripkeModel.models_axiomK;
 
-theorem kripke_sound' : Modal.K _ ⊢ φ → (∀ {κ}, [Nonempty κ] → ∀ M : KripkeModel κ α, M ⊧ φ)
-  := fun h {κ} [Nonempty κ] M ↦ kripke_sound h M.rel M.val
+theorem kripke_sound' : Modal.K _ ⊢ φ → (∀ κ, [Nonempty κ] → ∀ M : KripkeModel κ α, M ⊧ φ)
+  := fun h κ [Nonempty κ] M ↦ kripke_sound h κ M.frame M.val
 
 instance : Entailment.Consistent (Modal.K α) := by
   apply Hilbert.Normal.consistent_of_valid_model' (κ := Fin 1) (λ _ _ => True);
@@ -27,10 +26,10 @@ instance : Entailment.Consistent (Modal.K α) := by
   apply KripkeModel.models_axiomK;
 
 variable [DecidableEq α] [Encodable α] [Entailment.K (Modal.K α)]
-theorem kripke_complete : (∀ {κ : Type u}, [Nonempty κ] → ∀ M : KripkeModel κ α, M ⊧ φ) → Modal.K α ⊢ φ
-  := fun h ↦ canonicalKripkeModel.iff_valid_provable.mp $ h _
+theorem kripke_complete : (∀ κ : Type u, [Nonempty κ] → ∀ M : KripkeModel κ α, M ⊧ φ) → Modal.K _ ⊢ φ
+  := fun h ↦ canonicalKripkeModel.iff_valid_provable.mp $ h _ _
 
-theorem iff_provable_valid_all_kripkeModel : Modal.K α ⊢ φ ↔ (∀ {κ : Type u}, [Nonempty κ] → ∀ M : KripkeModel κ α, M ⊧ φ) := by
+theorem iff_provable_valid_all_kripkeModel : Modal.K _ ⊢ φ ↔ (∀ κ : Type u, [Nonempty κ] → ∀ M : KripkeModel κ α, M ⊧ φ) := by
   constructor;
   . apply kripke_sound';
   . apply kripke_complete;
